src/lists.lean
@@ -1,4 +1,5 @@
 import tactic
+import data.list.basic
 
 namespace list
 variables {α : Type*}
